simplified CM2 definition added problems   Two-counter Machine Reversibility (CM2_REV)   Reversible Two-counter Machine Halting (CM2_REV_HALT)   Two-counter Machine Uniform Boundedness (CM2_UBOUNDED)   Two-counter Machine Uniform Mortality (CM2_UMORTAL)   Two-counter (original) Minsky Machine Halting MM_2_HALTING added decision procedures   Two-counter Machine Reversibility (CM2_REV_dec.v)   Reversible Two-counter Machine Halting (CM2_REV_HALT_dec.v)   Two-counter Machine Uniform Boundedness (CM2_UBOUNDED_dec.v)   Two-counter Machine Uniform Mortality (CM2_UMORTAL_dec.v)   Two-counter (original) Minsky Machine Halting (MM_2_HALTING_dec.v) added top-level structure   Decidability Results on CM2 (CM2_dec.v)   Decidability Results on MM (MM2_dec.v)

theories/CounterMachines/CM2.v
@@ -2,19 +2,30 @@
   Autor(s):
     Andrej Dudenhefner (1) 
   Affiliation(s):
-    (1) Saarland University, Saarbrücken, Germany
+    (1) TU Dortmund University, Dortmund, Germany
 *)
 
 (* 
   Problem(s):
-    Two Counter Machine Halting (CM2_HALT)
+    Two-counter Machine Halting (CM2_HALT)
+    Two-counter Machine Reversibility (CM2_REV)
+    Reversible Two-counter Machine Halting (CM2_REV_HALT)
+    Two-counter Machine Uniform Boundedness (CM2_UBOUNDED)
+    Two-counter Machine Uniform Mortality (CM2_UMORTAL)
 *)
 
-Require Import List.
+Require Import List ssrfun.
 
-Definition State : Set := nat.
 (* a configuration consists of a state and two counter values *)
-Record Config : Set := mkConfig { state : State; value1 : nat; value2 : nat }.
+Definition Config : Set := nat * (nat * nat).
+
+(* accessors for state, value1, value2 of configurations *)
+Definition state (x: Config) : nat := fst x.
+Arguments state !x /.
+Definition value1 (x: Config) : nat := fst (snd x).
+Arguments value1 !x /.
+Definition value2 (x: Config) : nat := snd (snd x).
+Arguments value2 !x /.
 
 (* the instruction inc true maps 
       a configuration (p, (v1, v2)) to (1+p, (v1, 1+v2))
@@ -28,38 +39,94 @@ Record Config : Set := mkConfig { state : State; value1 : nat; value2 : nat }.
       a configuration (p, (1+v1, v2)) to (q, (v1, v2)) *)
 Inductive Instruction : Set := 
   | inc : bool -> Instruction
-  | dec : bool -> State -> Instruction.
+  | dec : bool -> nat -> Instruction.
 
-(* a two counter machine is a list of instructions *)
+(* a two-counter machine is a list of instructions *)
 Definition Cm2 : Set := list Instruction.
 
-(* two counter machine step function *)
-Definition step (M: Cm2) (x: Config) : Config :=
+(* partial two-counter machine step function *)
+Definition step (M: Cm2) (x: Config) : option Config :=
   match nth_error M (state x) with
-  | None => x (* halting configuration *)
+  | None => None (* halting configuration *)
   | Some (inc b) => (* increase counter, goto next state*)
-    {| state := 1 + (state x); 
-       value1 := (if b then 0 else 1) + (value1 x);
-       value2 := (if b then 1 else 0) + (value2 x) |}
+    Some (1 + (state x), ((if b then 0 else 1) + (value1 x), (if b then 1 else 0) + (value2 x)))
   | Some (dec b y) => (* decrease counter, if successful goto state y *)
-    if b then 
-      match value2 x with
-      | 0 => {| state := 1 + (state x); value1 := value1 x; value2 := 0 |}
-      | S n => {| state := y; value1 := value1 x; value2 := n |}
-      end
-    else
-      match value1 x with
-      | 0 => {| state := 1 + (state x); value1 := 0; value2 := value2 x |}
-      | S n => {| state := y; value1 := n; value2 := value2 x |}
-      end
+    Some (
+      if b then 
+        match value2 x with
+        | 0 => (1 + (state x), (value1 x, 0))
+        | S n => (y, (value1 x, n))
+        end
+      else
+        match value1 x with
+        | 0 => (1 + (state x), (0, value2 x))
+        | S n => (y, (n, value2 x))
+        end)
   end.
-(* unfold step if the configuration is decomposed *)
-Arguments step _ !x /.
 
-(* halting configuration property *)
-Definition halting (M : Cm2) (x: Config) : Prop := step M x = x.
+(* iterated partial two-counter machine step function *)
+Definition steps (M: Cm2) (k: nat) (x: Config) : option Config :=
+  Nat.iter k (obind (step M)) (Some x).
 
-(* Two Counter Machine Halting Problem *)
+(* two-counter machine configuration reachability *)
+Definition reaches (M: Cm2) (x y: Config) :=
+  exists k, steps M k x = Some y.
+
+(* does M eventually terminate starting from the configuration x? *)
+Definition terminating (M: Cm2) (x: Config) :=
+  exists k, steps M k x = None.
+
+(* injectivity of the step function *)
+Definition reversible (M : Cm2) : Prop := 
+  forall x y z, step M x = Some z -> step M y = Some z -> x = y.
+
+(* k bounds the number of reachable configurations from x *)
+Definition bounded (M: Cm2) (k: nat) (x: Config) : Prop := 
+  exists (L: list Config), (length L <= k) /\
+    (forall (y: Config), reaches M x y -> In y L).
+
+(* uniform bound for number of reachable configurations *)
+Definition uniformly_bounded (M: Cm2) : Prop :=
+  exists k, forall x, bounded M k x.
+
+(* k bounds the number of steps in a terminating run from x *)
+Definition mortal (M: Cm2) (k: nat) (x: Config) : Prop := 
+  steps M k x = None.
+
+(* uniform bound for number of steps until termination *)
+Definition uniformly_mortal (M: Cm2) : Prop :=
+  exists k, forall x, mortal M k x.
+
+(* Two-counter Machine Halting:
+   Given a two-counter machine M,
+   does a run in M starting from configuration (0, (0, 0)) eventually halt? *)
 Definition CM2_HALT : Cm2 -> Prop :=
-  fun M => exists (n: nat), 
-    halting M (Nat.iter n (step M) {| state := 0; value1 := 0; value2 := 0 |}).
+  fun M => terminating M (0, (0, 0)).
+
+(* Two-counter Machine Reversibility:
+   Given a two-counter machine M,
+   is the step function of M injective? *)
+Definition CM2_REV : Cm2 -> Prop :=
+  fun M => reversible M.
+
+(* Reversible Two-counter Machine Halting:
+   Given a reversible two-counter machine M and a configucation x, 
+   does a run in M starting from x eventually halt? *)
+Definition CM2_REV_HALT : { M: Cm2 | reversible M } * Config -> Prop :=
+  fun '((exist _ M _), x) => terminating M x.
+
+(* Two-counter Machine Uniform Boundedness:
+   Given a two-counter machine M,
+   is there a uniform bound n,
+   such that for any configuration x,
+   the number of reacheable configurations from x is bounded by n? *)
+Definition CM2_UBOUNDED : Cm2 -> Prop :=
+  fun M => uniformly_bounded M.
+
+(* Two-counter Machine Uniform Mortality:
+   Given a two-counter machine M,
+   is there a uniform bound n,
+   such that for any configuration x,
+   a run in M starting from x halts after at most n steps? *)
+Definition CM2_UMORTAL : Cm2 -> Prop :=
+  fun M => uniformly_mortal M.
